WIP Substitute everywhere

theories/Dot/syn/path_repl.v
@@ -23,28 +23,48 @@ Set Default Proof Using "Type".
 Notation unshift T := T.|[ren pred].
 Notation unshiftV v := v.[ren pred].
 
-Reserved Notation "p1 ~pp[ p := q  ] p2" (at level 70).
-Inductive path_path_repl (p q : path) : path → path → Prop :=
-| path_path_repl_base : p ~pp[ p := q ] q
-| path_path_repl_self p1 p2 l :
-  p1 ~pp[ p := q ] p2 →
-  pself p1 l ~pp[ p := q ] pself p2 l
-where "p1 ~pp[ p := q  ] p2" := (path_path_repl p q p1 p2) .
-
-(* Lemma path_path_repl_id p1 p2 p : p1 ~pp[ p := p ] p2 → p1 = p2.
-Proof. by elim; intros; simplify_eq/=. Qed. *)
-
-Notation path_path_repl_rtc p q := (rtc (path_path_repl p q)).
-Notation "p1 ~pp[ p := q  ]* p2" := (path_path_repl_rtc p q p1 p2) (at level 70).
-
-Reserved Notation "T1 ~Tp[ p := q  ] T2" (at level 70).
+Reserved Notation   "v1 ~vp[ p := q  ] v2"  (at level 70).
+Reserved Notation   "d1 ~dp[ p := q  ] d2"  (at level 70).
+Reserved Notation "ds1 ~dsp[ p := q  ] ds2" (at level 70).
+Reserved Notation   "p1 ~pp[ p := q  ] p2"  (at level 70).
+Reserved Notation   "T1 ~Tp[ p := q  ] T2"  (at level 70).
 
 (** ** The path replacement judgment, as defined in the pDOT paper.
 [T1 ~Tp[ p := q ] T2] means that [T2] is obtained from [T1] by replacing
 _one_ occurrence of [p] by [q]. We also use the reflexive-transitive closure
 of this judgemnt.
 *)
-Inductive ty_path_repl (p q : path) : ty → ty → Prop :=
+Inductive vl_path_repl (p q : path) : vl → vl → Prop :=
+| vl_path_repl_vobj ds1 ds2 :
+  ds1 ~dsp[ p := q ] ds2 →
+  vobj ds1 ~vp[ p := q ] vobj ds2
+where "v1 ~vp[ p := q  ] v2" := (vl_path_repl p q v1 v2)
+with dm_path_repl (p q : path) : dm → dm → Prop :=
+| dm_path_repl_dtysyn T1 T2 :
+  T1 ~Tp[ p := q ] T2 →
+  dtysyn T1 ~dp[ p := q ] dtysyn T2
+| dm_path_repl_dpt p1 p2 :
+  p1 ~pp[ p := q ] p2 →
+  dpt p1 ~dp[ p := q ] dpt p2
+where "d1 ~dp[ p := q  ] d2" := (dm_path_repl p q d1 d2)
+with dms_path_repl (p q : path) : dms → dms → Prop :=
+| dms_path_repl_cons1 l d1 d2 ds :
+  d1 ~dp[ p := q ] d2 →
+  (l, d1) :: ds ~dsp[ p := q ] (l, d2) :: ds
+| dms_path_repl_cons2 l d ds1 ds2 :
+  ds1 ~dsp[ p := q ] ds2 →
+  (l, d) :: ds1 ~dsp[ p := q ] (l, d) :: ds2
+where "ds1 ~dsp[ p := q  ] ds2" := (dms_path_repl p q ds1 ds2)
+with path_path_repl (p q : path) : path → path → Prop :=
+| path_path_repl_base : p ~pp[ p := q ] q
+| path_path_repl_pv v1 v2 :
+  v1 ~vp[ p := q ] v2 →
+  pv v1 ~pp[ p := q ] pv v2
+| path_path_repl_self p1 p2 l :
+  p1 ~pp[ p := q ] p2 →
+  pself p1 l ~pp[ p := q ] pself p2 l
+where "p1 ~pp[ p := q  ] p2" := (path_path_repl p q p1 p2)
+with ty_path_repl (p q : path) : ty → ty → Prop :=
 | ty_path_repl_TAnd1 T1 T2 U :
   T1 ~Tp[ p := q ] T2 →
   TAnd T1 U ~Tp[ p := q ] TAnd T2 U
@@ -86,8 +106,14 @@ Inductive ty_path_repl (p q : path) : ty → ty → Prop :=
   TSing p1 ~Tp[ p := q ] TSing p2
 where "T1 ~Tp[ p := q  ] T2" := (ty_path_repl p q T1 T2).
 
-Notation ty_path_repl_rtc p q := (rtc (ty_path_repl p q)).
-Notation "T1 ~Tp[ p := q  ]* T2" := (ty_path_repl_rtc p q T1 T2) (at level 70).
+(* Lemma path_path_repl_id p1 p2 p : p1 ~pp[ p := p ] p2 → p1 = p2.
+Proof. by elim; intros; simplify_eq/=. Qed. *)
+
+Notation   "v1 ~vp[ p := q  ]* v2"  := (rtc (vl_path_repl   p q) v1 v2)   (at level 70).
+Notation   "d1 ~dp[ p := q  ]* d2"  := (rtc (dm_path_repl   p q) d1  d2)  (at level 70).
+Notation "ds1 ~dsp[ p := q  ]* ds2" := (rtc (dms_path_repl  p q) ds1 ds2) (at level 70).
+Notation   "p1 ~pp[ p := q  ]* p2"  := (rtc (path_path_repl p q) p1 p2)   (at level 70).
+Notation   "T1 ~Tp[ p := q  ]* T2"  := (rtc (ty_path_repl   p q) T1 T2)   (at level 70).
 
 (* Lemma ty_path_repl_id p T1 T2 : T1 ~Tp[ p := p ] T2 → T1 = T2.
 Proof.
@@ -108,34 +134,27 @@ Notation "T .Tp[ p /]~ T'" := (path_repl_one T p T') (at level 65).
 We also define path replacement as a function, and prove it correct in
 [psubst_ty_rtc_sufficient].
 *)
+Reserved Notation "v .v[ p := q  ]" (at level 65).
+Reserved Notation "d .d[ p := q  ]" (at level 65).
 Reserved Notation "r .p[ p := q  ]" (at level 65).
-Fixpoint psubst_path p q r : path := match (decide (r = p)) with
-| left _ => q
-| _ =>
-  match r with
-  | pv _ => r
-  (* While these values can in turn contain paths, pDOT path replacement
-  doesn't substitute inside such values (because in pDOT such values cannot
-  appear in paths); lemma [psubst_path_rtc_sufficient] shows this
-  functional path replacement agrees with relational path replacement.
-
-  This operation is also used to build functional path substitution, for use
-  on unstamped types. And for unstamped types, lemma [psubst_one_implies]
-  shows this function is correct, relative to relational path substitution.
-
-  This design was chosen when values could not contain paths; now that values
-  _can_ contain paths, we could probably modify substitution to traverse
-  paths inside values.
-  *)
-  | pself r' l => pself (r' .p[ p := q ]) l
-  end
-end
-where "r .p[ p := q  ]" := (psubst_path p q r).
-(* Lemma psubst_path_self p q: p .p[ p := q ] = q.
-Proof. case: p => /= *; by rewrite decide_True. Qed. *)
-
 Reserved Notation "T .T[ p := q  ]" (at level 65).
-Fixpoint psubst_ty p q T : ty := match T with
+
+(* This still cannot substitute in dtysem, so we still need some
+unstampedness check, or just to forbid dtysem. *)
+Fixpoint psubst_vl p q v : vl :=
+  match v with
+  | vobj d => vobj (map (mapsnd (psubst_dm p q)) d)
+  | _ => v
+  end
+where "v .v[ p := q  ]" := (psubst_vl p q v)
+with psubst_dm p q d : dm :=
+  match d with
+  | dpt r => dpt (psubst_path p q r)
+  | dtysyn T => dtysyn (psubst_ty p q T)
+  | _ => d
+  end
+where "d .d[ p := q  ]" := (psubst_dm p q d)
+with psubst_ty p q T : ty := match T with
 | TTop => TTop
 | TBot => TBot
 | TAnd T1 T2 => TAnd (T1 .T[ p := q ]) (T2 .T[ p := q ])
@@ -149,7 +168,34 @@ Fixpoint psubst_ty p q T : ty := match T with
 | TPrim _ => T
 | TSing r => TSing (r .p[ p := q ])
 end
-where "T .T[ p := q  ]" := (psubst_ty p q T).
+where "T .T[ p := q  ]" := (psubst_ty p q T)
+with psubst_path p q r : path :=
+  match (decide (r = p)) with
+  | left _ => q
+  | _ =>
+    match r with
+    | pv v => pv (psubst_vl p q v)
+    | pself r' l => pself (r' .p[ p := q ]) l
+    end
+end
+where "r .p[ p := q  ]" := (psubst_path p q r).
+    (* XXX Update comment.
+    While these values can in turn contain paths, pDOT path replacement
+    doesn't substitute inside such values (because in pDOT such values cannot
+    appear in paths); lemma [psubst_path_rtc_sufficient] shows this
+    functional path replacement agrees with relational path replacement.
+
+    This operation is also used to build functional path substitution, for use
+    on unstamped types. And for unstamped types, lemma [psubst_one_implies]
+    shows this function is correct, relative to relational path substitution.
+
+    This design was chosen when values could not contain paths; now that values
+    _can_ contain paths, we could probably modify substitution to traverse
+    paths inside values.
+    *)
+
+(* Lemma psubst_path_self p q: p .p[ p := q ] = q.
+Proof. case: p => /= *; by rewrite decide_True. Qed. *)
 
 Section closure.
   Context `{RA : relation A} `{RB : relation B} `{RC : relation C}.
@@ -167,39 +213,69 @@ Section closure.
 End closure.
 
 Section decide_psubst.
-  Local Hint Constructors path_path_repl ty_path_repl : core.
+(** Instances of [rtc_congruence] where inference needs help. *)
+  Local Hint Constructors vl_path_repl dm_path_repl dms_path_repl
+    path_path_repl ty_path_repl : core.
 
-  (** Instances of [rtc_congruence] where inference needs help. *)
   Lemma path_path_repl_self_rtc p q p1 p2 l :
     p1 ~pp[ p := q ]* p2 →
     pself p1 l ~pp[ p := q ]* pself p2 l.
   Proof. apply rtc_congruence with (f := (λ p, pself p l)); auto. Qed.
 
-  Lemma ty_path_repl_TSel_rtc p1 q1 p q l :
-    p1 ~pp[ p := q ]* q1 →
-    TSel p1 l ~Tp[ p := q ]* TSel q1 l.
+  Lemma ty_path_repl_TSel_rtc p q p1 p2 l :
+    p1 ~pp[ p := q ]* p2 →
+    TSel p1 l ~Tp[ p := q ]* TSel p2 l.
   Proof. apply rtc_congruence with (f := (λ p, TSel p l)); auto. Qed.
 
+  Lemma dms_path_repl_cons_rtc p q l d1 d2 ds1 ds2 :
+    d1 ~dp[ p := q ]* d2 →
+    ds1 ~dsp[ p := q ]* ds2 →
+    (l, d1) :: ds1 ~dsp[ p := q ]* (l, d2) :: ds2.
+  Proof. eapply rtc_congruence2 with (f := λ d ds, (l, d) :: ds); auto. Qed.
+
   (** The reflexive, transitive closure of path replacement agrees with path
-  substitution. In fact, there can be only 0 or 1 steps anyway. *)
-  Lemma psubst_path_rtc_sufficient p1 q1 p q :
-    p1 .p[ p := q ] = q1 →
-    p1 ~pp[ p := q ]* q1.
+  substitution. *)
+
+  Notation psubst_rtc_sufficient_vl_def v1 := (∀ v2 p q,
+    v1 .v[ p := q ] = v2 → v1 ~vp[ p := q ]* v2).
+  Notation psubst_rtc_sufficient_dm_def d1 := (∀ d2 p q,
+    d1 .d[ p := q ] = d2 → d1 ~dp[ p := q ]* d2).
+  Notation psubst_rtc_sufficient_path_def p1 := (∀ p2 p q,
+    p1 .p[ p := q ] = p2 → p1 ~pp[ p := q ]* p2).
+  Notation psubst_rtc_sufficient_ty_def T1 := (∀ T2 p q,
+    T1 .T[ p := q ] = T2 → T1%ty ~Tp[ p := q ]* T2).
+
+  Lemma psubst_rtc_sufficient_mut :
+    (∀ t, True) ∧ (∀ v, psubst_rtc_sufficient_vl_def v) ∧
+    (∀ d, psubst_rtc_sufficient_dm_def d) ∧ (∀ p, psubst_rtc_sufficient_path_def p) ∧
+    (∀ T, psubst_rtc_sufficient_ty_def T).
   Proof.
-    intros; subst q1.
-    elim: p1 => [v|p1 IHp1 l] /=; case_decide as Hdec;
-      [ | done | | exact: path_path_repl_self_rtc];
-    rewrite Hdec; apply rtc_once; constructor.
+    apply syntax_mut_ind; intros; subst => //=;
+      try (case_decide as Hdec; first (rewrite Hdec; apply rtc_once; constructor));
+      eauto using rtc_refl, path_path_repl_self_rtc, ty_path_repl_TSel_rtc, rtc_congruence;
+      try by [eapply rtc_congruence2; eauto 2].
+
+    eapply rtc_congruence; first by eauto.
+    generalize dependent ds; elim => [//|[l d] ds IHds] /= /Forall_cons [Hd Hds].
+    by apply /dms_path_repl_cons_rtc /IHds /Hds /Hd.
   Qed.
 
+  Lemma psubst_vl_rtc_sufficient v1 v2 p q :
+    v1 .v[ p := q ] = v2 →
+    v1 ~vp[ p := q ]* v2.
+  Proof. apply psubst_rtc_sufficient_mut. Qed.
+  Lemma psubst_dm_rtc_sufficient d1 d2 p q :
+    d1 .d[ p := q ] = d2 →
+    d1 ~dp[ p := q ]* d2.
+  Proof. apply psubst_rtc_sufficient_mut. Qed.
+  Lemma psubst_path_rtc_sufficient p1 p2 p q :
+    p1 .p[ p := q ] = p2 →
+    p1 ~pp[ p := q ]* p2.
+  Proof. apply psubst_rtc_sufficient_mut. Qed.
   Lemma psubst_ty_rtc_sufficient T1 T2 p q :
     T1 .T[ p := q ] = T2 →
     T1 ~Tp[ p := q ]* T2.
-  Proof.
-    intros <-; move: p q.
-    induction T1; intros; simpl; eauto using rtc_congruence, rtc_congruence2,
-      ty_path_repl_TSel_rtc, psubst_path_rtc_sufficient, rtc_refl.
-  Qed.
+  Proof. apply psubst_rtc_sufficient_mut. Qed.
 End decide_psubst.
 
 (**
@@ -207,6 +283,10 @@ Finally, we can also define path substitution as a function.
 Its proofs of correctness is in [path_repl_lemmas.v], in lemmas
 [psubst_one_implies] and [psubst_subst_agree_ty].
 *)
+Definition psubst_one_base_vl v p := v .v[ pv (ids 0) := shift p ].
+Definition psubst_one_vl v p := unshiftV (psubst_one_base_vl v p).
+Notation "v .vp[ p /]" := (psubst_one_vl v p) (at level 65).
+
 Definition psubst_one_base_path q p := q .p[ pv (ids 0) := shift p ].
 Definition psubst_one_path q p := unshift (psubst_one_base_path q p).
 Notation "q .pp[ p /]" := (psubst_one_path q p) (at level 65).
@@ -214,3 +294,7 @@ Notation "q .pp[ p /]" := (psubst_one_path q p) (at level 65).
 Definition psubst_one_base_ty T p := T .T[ pv (ids 0) := shift p ].
 Definition psubst_one_ty T p := unshift (psubst_one_base_ty T p).
 Notation "T .Tp[ p /]" := (psubst_one_ty T p) (at level 65).
+
+Definition psubst_one_base_dm d p := d .d[ pv (ids 0) := shift p ].
+Definition psubst_one_dm d p := unshift (psubst_one_base_dm d p).
+Notation "d .dp[ p /]" := (psubst_one_dm d p) (at level 65).
